revised benchmarks

benchmarks/all.dfy
@@ -56,7 +56,7 @@ method BinarySearchWhile_Correct(a: array<int>, value: int) returns (index : int
 }
 
 method BubbleSort_Incorrect (a0: array<int>) returns (a: array<int>)
-  requires a0.Length >= 0 && a0.Length < 4
+  requires 0 <= a0.Length < 10
 	ensures sorted(a, 0, a.Length - 1) 
 {
     var i : int;
@@ -66,13 +66,13 @@ method BubbleSort_Incorrect (a0: array<int>) returns (a: array<int>)
     i := a.Length - 1;
 
 	while (i > 0)
-		invariant -1 <= i < a.Length && a.Length < 4
+		invariant -1 <= i < a.Length && a.Length < 10
 		invariant partitioned (a, 0, i, i+1, a.Length - 1)
 		invariant sorted (a, i, a.Length - 1)
 	{
 		j := 0;
 		while (j < i) 
-			invariant 1 <= i < a.Length && 0 <= j <= i && a.Length < 4
+			invariant 1 <= i < a.Length && 0 <= j <= i && a.Length < 10
 			invariant partitioned (a, 0, i, i + 1, a.Length - 1)
 			invariant partitioned (a, 0, j - 1, j, j)
 			invariant sorted (a, i, a.Length - 1)
@@ -87,7 +87,7 @@ method BubbleSort_Incorrect (a0: array<int>) returns (a: array<int>)
 }
 
 method BubbleSort_Correct (a0: array<int>) returns (a: array<int>)
-  requires a0.Length >= 0 && a0.Length < 4
+  requires 0 <= a0.Length < 10
 	ensures sorted(a, 0, a.Length - 1) 
 {
     var i : int;
@@ -97,14 +97,14 @@ method BubbleSort_Correct (a0: array<int>) returns (a: array<int>)
     i := a.Length - 1;
 
 	while (i > 0)
-		invariant -1 <= i < a.Length && a.Length < 4
+		invariant -1 <= i < a.Length && a.Length < 10
 		invariant i < 0 ==> a.Length == 0 
 		invariant partitioned (a, 0, i, i+1, a.Length - 1)
 		invariant sorted (a, i, a.Length - 1)
 	{
 		j := 0;
 		while (j < i) 
-			invariant 1 <= i < a.Length && 0 <= j <= i && a.Length < 4
+			invariant 1 <= i < a.Length && 0 <= j <= i && a.Length < 10
 			invariant partitioned (a, 0, i, i + 1, a.Length - 1)
 			invariant partitioned (a, 0, j - 1, j, j)
 			invariant sorted (a, i, a.Length - 1)
@@ -160,7 +160,7 @@ function Dist(x: int, y: int): int {
 }
 
 method CanyonSearch_Incorrect(a: array<int>, b: array<int>) returns (d: int)
-    requires a.Length > 0 && b.Length > 0 
+    requires 0 < a.Length <= 10 && 0 < b.Length <= 10
     requires sorted(a, 0, a.Length - 1) && sorted(b, 0, b.Length - 1)
     ensures exists i, j :: 0 <= i < a.Length && 0 <= j < b.Length && d == Dist(a[i], b[j])
     ensures forall i, j :: 0 <= i < a.Length && 0 <= j < b.Length ==> d <= Dist(a[i], b[j])
@@ -185,7 +185,7 @@ method CanyonSearch_Incorrect(a: array<int>, b: array<int>) returns (d: int)
 }
 
 method CanyonSearch_Correct(a: array<int>, b: array<int>) returns (d: int)
-    requires a.Length > 0 && b.Length > 0 
+    requires 0 < a.Length <= 10 && 0 < b.Length <= 10
     requires sorted(a, 0, a.Length - 1) && sorted(b, 0, b.Length - 1)
     ensures exists i, j :: 0 <= i < a.Length && 0 <= j < b.Length && d == Dist(a[i], b[j])
     ensures forall i, j :: 0 <= i < a.Length && 0 <= j < b.Length ==> d <= Dist(a[i], b[j])
@@ -220,7 +220,7 @@ predicate IsOdd(n: int)
 }
 
 method FirstEven_Incorrect(a: array<int>) returns (n: int)
-    requires a.Length >= 2 && a.Length <= 6
+    requires 2 <= a.Length <= 10
     requires exists i :: 0 <= i < a.Length && IsEven(a[i])
     ensures exists i :: 0 <= i < a.Length && IsEven(a[i]) && n == a[i] && (forall k :: 0 <= k < i ==> IsOdd(a[k]))
 {
@@ -233,8 +233,8 @@ method FirstEven_Incorrect(a: array<int>) returns (n: int)
         //invariant (0 <= firstEven < i) || firstEven == -1 //to be added
         invariant firstEven == -1 ==> (forall k :: 0 <= k < i ==> !IsEven(a[k]))
         invariant firstEven != -1 ==> (forall k :: 0 <= k < firstEven ==> IsOdd(a[k]))
-        /***************** Dafny doesn't need the below invariants *****************/
-        invariant a.Length >= 2 && a.Length <= 6
+        // dafny may not need these
+        invariant 2 <= a.Length <= 10
         invariant exists i :: 0 <= i < a.Length && IsEven(a[i])
         invariant firstEven != -1 && IsEven(a[i]) ==> firstEven == i 
         invariant forall k :: 0 <= k < i ==> IsOdd(a[k])
@@ -251,7 +251,7 @@ method FirstEven_Incorrect(a: array<int>) returns (n: int)
 
 
 method FirstEven_Correct(a: array<int>) returns (n: int)
-    requires a.Length >= 2 && a.Length <= 6
+    requires 2 <= a.Length <= 10
     requires exists i :: 0 <= i < a.Length && IsEven(a[i])
     ensures exists i :: 0 <= i < a.Length && IsEven(a[i]) && n == a[i] && (forall k :: 0 <= k < i ==> IsOdd(a[k]))
 {
@@ -263,8 +263,8 @@ method FirstEven_Correct(a: array<int>) returns (n: int)
         invariant (firstEven == -1 || (0 <= firstEven && firstEven < i && IsEven(a[firstEven]))) //correct invariant
         invariant firstEven == -1 ==> (forall k :: 0 <= k < i ==> !IsEven(a[k]))
         invariant firstEven != -1 ==> (forall k :: 0 <= k < firstEven ==> IsOdd(a[k]))
-        /***************** Dafny doesn't need the below invariants *****************/
-        invariant a.Length >= 2 && a.Length <= 6
+        // dafny may not need these
+        invariant 2 <= a.Length <= 10
         invariant exists i :: 0 <= i < a.Length && IsEven(a[i])
         invariant firstEven != -1 && IsEven(a[i]) ==> firstEven == i 
         invariant forall k :: 0 <= k < i ==> IsOdd(a[k])
@@ -280,7 +280,7 @@ method FirstEven_Correct(a: array<int>) returns (n: int)
 }
 
 method FirstEvenOddDifference_Incorrect (a: array<int>) returns (diff: int)
-    requires a.Length >= 2 && a.Length <= 6
+    requires 2 <= a.Length <= 10
     requires exists i :: 0 <= i < a.Length && IsEven(a[i])
     requires exists i :: 0 <= i < a.Length && IsOdd(a[i])
     ensures exists i, j :: 0 <= i < a.Length && 0 <= j < a.Length && IsEven(a[i]) && IsOdd(a[j]) && diff == a[i] - a[j] && 
@@ -294,14 +294,14 @@ method FirstEvenOddDifference_Incorrect (a: array<int>) returns (diff: int)
         invariant 0 <= i <= a.Length
         invariant 0 <= firstEven < i ==> IsEven(a[firstEven]) //wrong invariant 
         //invariant (0 <= firstEven && firstEven < i) || firstEven == -1 // to be added
-        invariant (firstOdd == -1 || (0 <= firstOdd && firstOdd < i && IsOdd(a[firstOdd]))) // 위와 마찬가지
+        invariant (firstOdd == -1 || (0 <= firstOdd && firstOdd < i && IsOdd(a[firstOdd])))
         //invariant 0 <= firstOdd && firstOdd < i ==> IsOdd(a[firstOdd]) 
         invariant firstEven == -1 ==> (forall k :: 0 <= k < i ==> !IsEven(a[k]))
         invariant firstOdd == -1 ==> (forall k :: 0 <= k < i ==> !IsOdd(a[k]))
         invariant firstEven != -1 ==> (forall k :: 0 <= k < firstEven ==> IsOdd(a[k]))
         invariant firstOdd != -1 ==> (forall k :: 0 <= k < firstOdd ==> IsEven(a[k]))
-        /***************** Dafny doesn't need the below invariants *****************/
-        invariant a.Length >= 2 && a.Length <= 6
+        // dafny may not need these
+        invariant 2 <= a.Length <= 10
         invariant exists i :: 0 <= i < a.Length && IsEven(a[i]) 
         invariant exists i :: 0 <= i < a.Length && IsOdd(a[i]) 
         invariant firstEven != -1 && firstOdd != -1 ==> ((firstEven < firstOdd ==> i == firstOdd) && (firstOdd < firstEven ==> i == firstEven)) 
@@ -325,7 +325,7 @@ method FirstEvenOddDifference_Incorrect (a: array<int>) returns (diff: int)
 
 
 method FirstEvenOddDifference_Correct (a: array<int>) returns (diff: int)
-    requires a.Length >= 2 && a.Length <= 6
+    requires 2 <= a.Length <= 10
     requires exists i :: 0 <= i && i < a.Length && IsEven(a[i])
     requires exists i :: 0 <= i && i < a.Length && IsOdd(a[i])
     ensures exists i, j :: 0 <= i && i < a.Length && 0 <= j && j < a.Length && IsEven(a[i]) && IsOdd(a[j]) && diff == a[i] - a[j] && 
@@ -343,8 +343,8 @@ method FirstEvenOddDifference_Correct (a: array<int>) returns (diff: int)
         invariant firstOdd == -1 ==> (forall k :: 0 <= k && k < i ==> !IsOdd(a[k]))
         invariant firstEven != -1 ==> (forall k :: 0 <= k && k < firstEven ==> IsOdd(a[k]))
         invariant firstOdd != -1 ==> (forall k :: 0 <= k && k < firstOdd ==> IsEven(a[k]))
-        /***************** Dafny doesn't need the below invariants *****************/
-        invariant a.Length >= 2 && a.Length <= 6
+        // dafny may not need these
+        invariant 2 <= a.Length <= 10
         invariant exists i :: 0 <= i < a.Length && IsEven(a[i]) 
         invariant exists i :: 0 <= i < a.Length && IsOdd(a[i]) 
         invariant firstEven != -1 && firstOdd != -1 ==> ((firstEven < firstOdd ==> i == firstOdd) && (firstOdd < firstEven ==> i == firstEven)) 
@@ -378,7 +378,7 @@ function random (l: int, u: int) : int
 }
 
 method InsertionSort_Incorrect1(a0:array<int>) returns (a:array<int>)
-  requires 5 >= a0.Length >= 2 
+  requires 2 <= a0.Length <= 10
   ensures sorted(a, 0, a.Length-1)
 {
   var x : int := 1;
@@ -389,19 +389,17 @@ method InsertionSort_Incorrect1(a0:array<int>) returns (a:array<int>)
   while (x < a.Length)
     invariant 1 <= x <= a.Length
     invariant sorted(a, 0, x-1)
-
     //dafny may not need these
-    invariant 5 >= a0.Length >= 2
+    invariant 2 <= a0.Length <= 10
   {
     d := x;
     while (d >= 1 andalso a[d-1] > a[d])
       invariant 0 <= d <= x
       invariant forall i,j :: 0 <= i < j < d ==> a[i] <= a[j] //wrong
       //invariant forall i,j ::( 0 <= i < j <= x && j != d) ==> a[i] <= a[j]  //correct
-
       //dafny may not need these
-      invariant 5 >= a0.Length >= 2
-      invariant 1 <= x < a.Length // took some time to figure out
+      invariant 2 <= a0.Length <= 5 
+      invariant 1 <= x < a.Length 
     {
       a[d-1], a[d] := a[d], a[d-1];
       d := d-1;
@@ -410,9 +408,8 @@ method InsertionSort_Incorrect1(a0:array<int>) returns (a:array<int>)
   }
 }
 
-method InsertionSort_Incorect2(a0:array<int>) returns (a:array<int>)
-  //modifies a
-  requires 5 >= a0.Length >= 2 
+method InsertionSort_Incorrect2(a0:array<int>) returns (a:array<int>)
+  requires 2 <= a0.Length <= 10
   ensures sorted(a, 0, a.Length-1)
 {
   var x : int := 1;
@@ -423,18 +420,16 @@ method InsertionSort_Incorect2(a0:array<int>) returns (a:array<int>)
   while (x < a.Length)
     invariant 1 <= x <= a.Length
     invariant sorted(a, 0, x-1)
-
     //dafny may not need these
-    invariant 5 >= a0.Length >= 2
+    invariant 2 <= a0.Length <= 10 
   {
     d := x;
     while (d >= 1 andalso a[d-1] > a[d])
       invariant 0 <= d <= x
       invariant forall i,j :: 0 <= i < j <= x /* && j != d */ ==> a[i] <= a[j]
-
       //dafny may not need these
-      invariant 5 >= a0.Length >= 2
-      invariant 1 <= x < a.Length // took some time to figure out
+      invariant 2 <= a0.Length <= 10 
+      invariant 1 <= x < a.Length 
     {
       a[d-1], a[d] := a[d], a[d-1];
       d := d-1;
@@ -444,7 +439,7 @@ method InsertionSort_Incorect2(a0:array<int>) returns (a:array<int>)
 }
 
 method InsertionSort_Correct(a0:array<int>) returns (a:array<int>)
-  requires 5 >= a0.Length >= 2 
+  requires 2 <= a0.Length <= 10
   ensures sorted(a, 0, a.Length-1)
 {
   var x : int := 1;
@@ -455,19 +450,16 @@ method InsertionSort_Correct(a0:array<int>) returns (a:array<int>)
   while (x < a.Length)
     invariant 1 <= x <= a.Length
     invariant sorted(a, 0, x-1)
-
     //dafny may not need these
-    invariant 5 >= a0.Length >= 2
+    invariant 2 <= a0.Length <= 10 
   {
     d := x;
     while (d >= 1 andalso a[d-1] > a[d])
       invariant 0 <= d <= x
-      // invariant forall i,j :: 0 <= i < j < d ==> a[i] <= a[j] //wrong
-      invariant forall i,j ::( 0 <= i < j <= x && j != d) ==> a[i] <= a[j]  //correct
-
+      invariant forall i,j ::( 0 <= i < j <= x && j != d) ==> a[i] <= a[j]
       //dafny may not need these
-      invariant 5 >= a0.Length >= 2
-      invariant 1 <= x < a.Length // took some time to figure out
+      invariant 2 <= a0.Length <= 10
+      invariant 1 <= x < a.Length 
     {
       a[d-1], a[d] := a[d], a[d-1];
       d := d-1;
@@ -477,7 +469,7 @@ method InsertionSort_Correct(a0:array<int>) returns (a:array<int>)
 }
 
 method IsPalindrome_Incorrect(x: array<int>) returns (result: bool)
-  requires x.Length >= 0
+  requires 0 <= x.Length
   ensures result <==> (forall i :: 0 <= i < x.Length  ==> x[i] == x[x.Length - i - 1])
 {
   var i :int := 0;
@@ -490,9 +482,8 @@ method IsPalindrome_Incorrect(x: array<int>) returns (result: bool)
   result := true;
   while (i < j)
     invariant 0 <= i <= j+1 && 0 <= j < x.Length 
-    //invariant i + j == x.Length -1 //when omitted, the third invariant & postconditon are not proved
+    //invariant i + j == x.Length -1
     invariant forall k :: 0 <= k < i ==> x[k] == x[x.Length - k - 1]
-
     // dafny doesn't need these
     invariant result == false ==> (exists k :: 0 <= k < x.Length && x[k] != x[x.Length - k - 1])
   {
@@ -506,7 +497,7 @@ method IsPalindrome_Incorrect(x: array<int>) returns (result: bool)
 }
 
 method IsPalindrome_Correct(x: array<int>) returns (result: bool)
-  requires x.Length >= 0
+  requires 0 <= x.Length 
   ensures result <==> (forall i :: 0 <= i < x.Length  ==> x[i] == x[x.Length - i - 1])
 {
   var i :int := 0;
@@ -519,9 +510,8 @@ method IsPalindrome_Correct(x: array<int>) returns (result: bool)
   result := true;
   while (i < j)
     invariant 0 <= i <= j+1 && 0 <= j < x.Length 
-    invariant i + j == x.Length -1 //when omitted, the third invariant & postconditon are not proved
+    invariant i + j == x.Length -1 
     invariant forall k :: 0 <= k < i ==> x[k] == x[x.Length - k - 1]
-
     // dafny doesn't need these
     invariant result == false ==> (exists k :: 0 <= k < x.Length && x[k] != x[x.Length - k - 1])
   {
@@ -536,12 +526,11 @@ method IsPalindrome_Correct(x: array<int>) returns (result: bool)
 
 
 method LucidNumbers_Incorrect(n: int) returns (lucid: array<int>)
-    requires n >= 0
+    requires 0 <= n 
     ensures forall i :: 0 <= i < lucid.Length ==> lucid[i] % 3 == 0
     ensures forall i :: 0 <= i < lucid.Length ==> lucid[i] <= n
     ensures forall i, j :: 0 <= i < j < lucid.Length ==> lucid[i] < lucid[j]
 {
-    // Allocate array with the maximum size needed for multiples of 3
     var maxSize : int := n / 3 + 1;
     var index : int := 0;
     var i : int := 0;
@@ -555,12 +544,11 @@ method LucidNumbers_Incorrect(n: int) returns (lucid: array<int>)
         invariant forall j1 :: 0 <= j1 < index ==> lucid[j1] % 3 == 0
         invariant forall j2 :: 0 <= j2 < index ==> lucid[j2] <= i /* -1 */ 
         invariant forall j3, k :: 0 <= j3 < k < index ==> lucid[j3] < lucid[k]
-
         //dafny doesn't need the below invariants
         invariant lucid.Length == maxSize
     {
         if (i % 3 == 0) {
-            if (index < maxSize) {  // Ensure index does not exceed the array bounds
+            if (index < maxSize) {  
                 lucid[index] := i;
                 index := index + 1;
             }
@@ -568,8 +556,6 @@ method LucidNumbers_Incorrect(n: int) returns (lucid: array<int>)
         i := i + 1;
     }
 
-    // Resize the array to fit the exact number of elements
-    
     resized := new [index];
     j := 0;
     while (j < index)
@@ -577,9 +563,8 @@ method LucidNumbers_Incorrect(n: int) returns (lucid: array<int>)
         invariant forall k :: 0 <= k < j ==> resized[k] == lucid[k]
         invariant forall i :: 0 <= i < index ==> lucid[i] % 3 == 0
         invariant forall i :: 0 <= i < index ==> lucid[i] <= n
-        invariant forall i, j4 :: 0 <= i < j4 < index ==> lucid[i] < lucid[j4] 
-        
-        //dafny doesn't need the below invariants
+        invariant forall i, j4 :: 0 <= i < j4 < index ==> lucid[i] < lucid[j4]  
+        // dafny may not need these
         invariant lucid.Length == maxSize
         invariant resized.Length == index
     {
@@ -592,12 +577,11 @@ method LucidNumbers_Incorrect(n: int) returns (lucid: array<int>)
 
 
 method LucidNumbers_Correct(n: int) returns (lucid: array<int>)
-    requires n >= 0
+    requires 0 <= n
     ensures forall i :: 0 <= i < lucid.Length ==> lucid[i] % 3 == 0
     ensures forall i :: 0 <= i < lucid.Length ==> lucid[i] <= n
     ensures forall i, j :: 0 <= i < j < lucid.Length ==> lucid[i] < lucid[j]
 {
-    // Allocate array with the maximum size needed for multiples of 3
     var maxSize : int := n / 3 + 1;
     var index : int := 0;
     var i : int := 0;
@@ -611,20 +595,17 @@ method LucidNumbers_Correct(n: int) returns (lucid: array<int>)
         invariant forall j1 :: 0 <= j1 < index ==> lucid[j1] % 3 == 0
         invariant forall j2 :: 0 <= j2 < index ==> lucid[j2] <= i - 1 
         invariant forall j3, k :: 0 <= j3 < k < index ==> lucid[j3] < lucid[k]
-
-        //dafny doesn't need the below invariants
+        // dafny may not need these
         invariant lucid.Length == maxSize
     {
         if (i % 3 == 0) {
-            if (index < maxSize) {  // Ensure index does not exceed the array bounds
+            if (index < maxSize) {  
                 lucid[index] := i;
                 index := index + 1;
             }
         }
         i := i + 1;
     }
-
-    // Resize the array to fit the exact number of elements
     
     resized := new [index];
     j := 0;
@@ -634,7 +615,6 @@ method LucidNumbers_Correct(n: int) returns (lucid: array<int>)
         invariant forall i :: 0 <= i < index ==> lucid[i] % 3 == 0
         invariant forall i :: 0 <= i < index ==> lucid[i] <= n
         invariant forall i, j4 :: 0 <= i < j4 < index ==> lucid[i] < lucid[j4] 
-        
         //dafny doesn't need the below invariants
         invariant lucid.Length == maxSize
         invariant resized.Length == index
@@ -645,7 +625,6 @@ method LucidNumbers_Correct(n: int) returns (lucid: array<int>)
     lucid := resized;
     
 }
-
 
 
 method Partition_Incorrect(a0: array<int>, l: int, u: int) returns (pivot: int, a: array<int>)
@@ -747,7 +726,7 @@ method ReverseUptoK_Incorrect (s_in: array<int>, k: int) returns (s : array<int>
         //to be added: invariant forall p :: (l - i < p && p <= l) ==> s[p] == s_in[l-p]
 		    invariant forall p :: i <= p <= l - i ==> s[p] == s_in[p]
         invariant forall p :: k <= p < s.Length ==> s[p] == s_in[p]
-        /********** Dafny doesn't need the invariants below **********/
+        // dafny may not need these
         invariant 2 <= k <= s.Length 
         invariant l == k - 1 
 	  {
@@ -774,7 +753,7 @@ method ReverseUptoK_Correct (s_in: array<int>, k: int) returns (s : array<int>)
 		    invariant forall p :: (0 <= p < i) || (l - i < p <= l) ==> s[p] == s_in[l-p]
 		    invariant forall p :: i <= p <= l - i ==> s[p] == s_in[p]
         invariant forall p :: k <= p < s.Length ==> s[p] == s_in[p]
-        /********** Dafny doesn't need the invariants below **********/
+        // dafny may not need these
         invariant 2 <= k <= s.Length 
         invariant l == k - 1 
 	  {
@@ -788,7 +767,7 @@ method ReverseUptoK_Correct (s_in: array<int>, k: int) returns (s : array<int>)
 
 
 method SelectionSort1_Incorrect (a0: array<int>) returns (a: array<int>)
-	  requires a0.Length >= 0
+	  requires 0 <= a0.Length 
 	  ensures sorted(a, 0, a.Length - 1)
 {
 	  var i : int := 0;
@@ -823,7 +802,7 @@ method SelectionSort1_Incorrect (a0: array<int>) returns (a: array<int>)
 }
 
 method SelectionSort1_Correct (a0: array<int>) returns (a: array<int>)
-	  requires a0.Length >= 0
+	  requires 0 <= a0.Length 
 	  ensures sorted(a, 0, a.Length - 1)
 {
 	  var i : int := 0;
@@ -858,7 +837,7 @@ method SelectionSort1_Correct (a0: array<int>) returns (a: array<int>)
 
 
 method SumOfSquaresOfFirstNOddNumbers_Incorrect (n: int) returns (sum: int)
-    requires n >= 0
+    requires 0 <= n
     ensures sum == (n * (2 * n - 1) * (2 * n + 1)) / 3
 {
     var i : int := 1;
@@ -877,7 +856,7 @@ method SumOfSquaresOfFirstNOddNumbers_Incorrect (n: int) returns (sum: int)
 }
 
 method SumOfSquaresOfFirstNOddNumbers_Correct (n: int) returns (sum: int)
-    requires n >= 0
+    requires 0 <= n
     ensures sum == (n * (2 * n - 1) * (2 * n + 1)) / 3
 {
     var i : int := 1;
@@ -895,4 +874,544 @@ method SumOfSquaresOfFirstNOddNumbers_Correct (n: int) returns (sum: int)
     }
 }
 
+method InvertArray_Incorrect(a0: array<int>) returns (a: array<int>)
+    requires 0 <= a0.Length <= 10
+    ensures forall i :: 0 <= i < a.Length ==> a[i] == a0[a.Length - 1 - i]
+    ensures a.Length == a0.Length
+{
+    var index:int := 0;
+    a := a0;
 
+    while (index < a.Length / 2)
+        invariant 0 <= index <= a.Length / 2
+        invariant forall i :: 0 <= i < index ==> a[i] == a0[a.Length - 1 - i]
+        invariant forall i :: 0 <= i < index ==> a[a.Length - 1 - i] == a0[i]
+        //invariant forall i :: index <= i < a.Length - index ==> a[i] == a0[i]
+        // dafny may not need these
+        invariant 0 <= a0.Length <= 10
+        invariant a.Length == a0.Length
+    {
+        a[index], a[a.Length - 1 - index] := a[a.Length - 1 - index], a[index];
+        index := index + 1;
+    }
+}
+
+method InvertArray_Correct(a0: array<int>) returns (a: array<int>)
+    requires 0 <= a0.Length <= 10
+    ensures forall i :: 0 <= i < a.Length ==> a[i] == a0[a.Length - 1 - i]
+    ensures a.Length == a0.Length
+{
+    var index:int := 0;
+    a := a0;
+
+    while (index < a.Length / 2)
+        invariant 0 <= index <= a.Length / 2
+        invariant forall i :: 0 <= i < index ==> a[i] == a0[a.Length - 1 - i]
+        invariant forall i :: 0 <= i < index ==> a[a.Length - 1 - i] == a0[i]
+        invariant forall i :: index <= i < a.Length - index ==> a[i] == a0[i]
+        // dafny may not need these
+        invariant 0 <= a0.Length <= 10
+        invariant a.Length == a0.Length
+    {
+        a[index], a[a.Length - 1 - index] := a[a.Length - 1 - index], a[index];
+        index := index + 1;
+    }
+}
+
+predicate odd (n: int) { n % 2 == 1 }
+predicate even (n: int) { n % 2 == 0 }
+
+method PartitionOddEven_Incorrect(a0: array<int>) returns (a: array<int>)
+    requires 0 <= a0.Length <= 10
+    ensures !(exists i, j :: 0 <= i < j < a.Length && even(a[i]) && odd(a[j]))
+{
+    var i : int := 0;
+    var j : int := a0.Length - 1; 
+
+    a := a0;
+    while (i <= j)
+        invariant 0 <= i <= j + 1 <= a.Length
+        invariant forall k :: 0 <= k < i ==> odd(a[k])
+        invariant forall k :: j <= k < a.Length ==> even(a[k]) 
+    {
+        if (even(a[i]) andalso odd(a[j])) { a[i], a[j] := a[j], a[i]; }
+        if (odd(a[i])) { i := i + 1; }
+        if (even(a[j])) { j := j - 1; }
+    }
+}
+
+method PartitionOddEven_Correct(a0: array<int>) returns (a: array<int>)
+    requires 0 <= a0.Length <= 10
+    ensures !(exists i, j :: 0 <= i < j < a.Length && even(a[i]) && odd(a[j]))
+{
+    var i : int := 0;
+    var j : int := a0.Length - 1; 
+
+    a := a0;
+    while (i <= j)
+        invariant 0 <= i <= j + 1 <= a.Length
+        invariant forall k :: 0 <= k < i ==> odd(a[k])
+        invariant forall k :: j < k < a.Length ==> even(a[k]) 
+     {
+        if (even(a[i]) andalso odd(a[j])) { a[i], a[j] := a[j], a[i]; }
+        if (odd(a[i])) { i := i + 1; }
+        if (even(a[j])) { j := j - 1; }
+    }
+}
+
+method Union_Incorrect(a: array<int>, b: array<int>) returns (u: array<int>)
+    requires 0 <= a.Length <= 10 && 0 <= b.Length <= 10
+    ensures u.Length == a.Length + b.Length 
+    ensures forall i :: 0 <= i < a.Length ==> u[i] == a[i] 
+    ensures forall i :: 0 <= i < b.Length ==> u[a.Length + i] == b[i] 
+{
+    var j : int;
+    var i : int;
+
+    j := 0;
+    i := 0;
+    u := new [a.Length + b.Length];
+
+    while (i < a.Length)
+        invariant 0 <= i <= a.Length
+        invariant 0 <= j <= a.Length
+        invariant forall k :: 0 <= k < i ==> u[k] == a[k]
+        invariant i == j
+        // dafny may not need these
+        invariant u.Length == a.Length + b.Length 
+        invariant 0 <= a.Length <= 10 && 0 <= b.Length <= 10
+    {
+        u[j] := a[i];
+        j := j + 1;
+        i := i + 1;
+    }
+    
+    i := 0;
+
+    while (i < b.Length)
+        invariant 0 <= i <= b.Length
+        invariant a.Length <= j <= u.Length
+        invariant forall k :: a.Length <= k < j ==> u[k] == b[k - a.Length]
+        //invariant forall k :: 0 <= k < a.Length ==> u[k] == a[k] 
+        invariant i == j - a.Length 
+        // dafny may not need these
+        invariant u.Length == a.Length + b.Length 
+        invariant 0 <= a.Length <= 10 && 0 <= b.Length <= 10
+    {
+        u[j] := b[i];
+        j := j + 1;
+        i := i + 1;
+    }
+}
+
+
+method Union_Correct(a: array<int>, b: array<int>) returns (u: array<int>)
+    requires 0 <= a.Length <= 10 && 0 <= b.Length <= 10
+    ensures u.Length == a.Length + b.Length 
+    ensures forall i :: 0 <= i < a.Length ==> u[i] == a[i] 
+    ensures forall i :: 0 <= i < b.Length ==> u[a.Length + i] == b[i] 
+{
+    var j : int;
+    var i : int;
+
+    j := 0;
+    i := 0;
+    u := new [a.Length + b.Length];
+
+    while (i < a.Length)
+        invariant 0 <= i <= a.Length
+        invariant 0 <= j <= a.Length
+        invariant forall k :: 0 <= k < i ==> u[k] == a[k]
+        invariant i == j
+        // dafny may not need these
+        invariant u.Length == a.Length + b.Length 
+        invariant 0 <= a.Length <= 10 && 0 <= b.Length <= 10
+    {
+        u[j] := a[i];
+        j := j + 1;
+        i := i + 1;
+    }
+    
+    i := 0;
+
+    while (i < b.Length)
+        invariant 0 <= i <= b.Length
+        invariant a.Length <= j <= u.Length
+        invariant forall k :: a.Length <= k < j ==> u[k] == b[k - a.Length]
+        invariant forall k :: 0 <= k < a.Length ==> u[k] == a[k] 
+        invariant i == j - a.Length 
+        // dafny may not need these
+        invariant u.Length == a.Length + b.Length 
+        invariant 0 <= a.Length <= 10 && 0 <= b.Length <= 10
+    {
+        u[j] := b[i];
+        j := j + 1;
+        i := i + 1;
+    }
+}
+
+method FindFirstRepeatedInt_Incorrect(s: array<int>) returns (found: bool, c: int)
+    requires 0 <= s.Length <= 10
+    ensures found ==> exists i, j :: 0 <= i < j < s.Length && s[i] == s[j] && s[i] == c && (forall k, l :: 0 <= k < l < j && s[k] == s[l] ==> k >= i)
+    ensures !found ==> (forall i, j :: 0 <= i < j < s.Length ==> s[i] != s[j])
+{
+    var inner_found: bool := false;
+    var i: int := 0;
+    var j: int;
+    c := -1;
+    found := false;
+
+    while (i < s.Length andalso (found == false))
+        invariant 0 <= i <= s.Length 
+        // invariant found == inner_found
+        invariant found ==> exists ii, jj :: 0 <= ii < i && ii < jj < s.Length && s[ii] == s[jj] && s[ii] == c && (forall k, l :: 0 <= k < l < jj && s[k] == s[l] ==> k >= ii)
+        invariant !found ==> (forall ii, jj :: 0 <= ii < i && ii < jj < s.Length ==> s[ii] != s[jj])
+    {
+        j := i + 1;
+
+        while (j < s.Length andalso (inner_found == false))
+            invariant i < j <= s.Length 
+            invariant inner_found ==> exists k :: i < k < s.Length && s[i] == s[k] && s[i] == c 
+            invariant !inner_found ==> (forall k :: i < k < j ==> s[i] != s[k]) 
+            // dafny may not need these
+            invariant 0 <= i <= s.Length
+            invariant found ==> inner_found
+            invariant found ==> exists ii, jj :: 0 <= ii < i && ii < jj < s.Length && s[ii] == s[jj] && s[ii] == c && (forall k, l :: 0 <= k < l < jj && s[k] == s[l] ==> k >= ii)
+            invariant !found ==> (forall ii, jj :: 0 <= ii < i && ii < jj < s.Length ==> s[ii] != s[jj])
+        {
+            if (s[i] == s[j]) {
+                inner_found := true;
+                c := s[i];
+            }
+            j := j + 1;
+        }
+        found := inner_found;
+        i := i + 1;
+    }
+}
+
+method FindFirstRepeatedInt_Correct(s: array<int>) returns (found: bool, c: int)
+    requires 0 <= s.Length <= 10
+    ensures found ==> exists i, j :: 0 <= i < j < s.Length && s[i] == s[j] && s[i] == c && (forall k, l :: 0 <= k < l < j && s[k] == s[l] ==> k >= i)
+    ensures !found ==> (forall i, j :: 0 <= i < j < s.Length ==> s[i] != s[j])
+{
+    var inner_found: bool := false;
+    var i: int := 0;
+    var j: int;
+    c := -1;
+    found := false;
+
+    while (i < s.Length andalso (found == false))
+        invariant 0 <= i <= s.Length 
+        invariant found == inner_found
+        invariant found ==> exists ii, jj :: 0 <= ii < i && ii < jj < s.Length && s[ii] == s[jj] && s[ii] == c && (forall k, l :: 0 <= k < l < jj && s[k] == s[l] ==> k >= ii)
+        invariant !found ==> (forall ii, jj :: 0 <= ii < i && ii < jj < s.Length ==> s[ii] != s[jj])
+    {
+        j := i + 1;
+
+        while (j < s.Length andalso (inner_found == false))
+            invariant i < j <= s.Length 
+            invariant inner_found ==> exists k :: i < k < s.Length && s[i] == s[k] && s[i] == c 
+            invariant !inner_found ==> (forall k :: i < k < j ==> s[i] != s[k]) 
+            // dafny may not need these
+            invariant 0 <= i <= s.Length
+            invariant found ==> inner_found
+            invariant found ==> exists ii, jj :: 0 <= ii < i && ii < jj < s.Length && s[ii] == s[jj] && s[ii] == c && (forall k, l :: 0 <= k < l < jj && s[k] == s[l] ==> k >= ii)
+            invariant !found ==> (forall ii, jj :: 0 <= ii < i && ii < jj < s.Length ==> s[ii] != s[jj])
+        {
+            if (s[i] == s[j]) {
+                inner_found := true;
+                c := s[i];
+            }
+            j := j + 1;
+        }
+        found := inner_found;
+        i := i + 1;
+    }
+}
+
+predicate strictSorted(s : array<int>) 
+{
+	forall i, j :: 0 <= i < j < s.Length ==> s[i] < s[j] 
+}
+
+method mContained_Incorrect(v:array<int>,w:array<int>,n:int,m:int) returns (b:bool)
+    requires n <= m && n >= 0
+    requires strictSorted(v)
+    requires strictSorted(w)
+    requires v.Length >= n && w.Length >= m
+    requires v.Length <= 10 && w.Length <= 10
+    ensures b <==> forall k:: 0 <= k < n ==> exists x :: 0 <= x < m && v[k] == w[x]
+{
+	  var i: int := 0;
+	  var j: int := 0;
+
+	  while (i < n andalso j < m andalso (v[i] >= w[j]))
+	      invariant 0 <= i <= n
+	      invariant 0 <= j <= m
+        invariant forall k :: 0 <= k < i ==> (exists x:: 0 <= x < j && v[k] == w[x]) 
+	      //invariant i < n ==> !(exists x:: 0 <= x < j && v[i] == w[x]) 
+        // dafny may not need these
+        invariant strictSorted(v)
+	      invariant strictSorted(w)
+        invariant n <= m && n >= 0
+        invariant v.Length >= n && w.Length >= m
+	  {	
+	  	  if(v[i] == w[j]){
+	  	  	i:=i+1;
+	  	  }
+	  	  j:=j+1;
+	  }
+
+    if (i == n){
+        b := true;
+    }
+    else{
+        b := false;
+    }
+}
+
+method mContained_Correct(v:array<int>,w:array<int>,n:int,m:int) returns (b:bool)
+    requires n <= m && n >= 0
+    requires strictSorted(v)
+    requires strictSorted(w)
+    requires v.Length >= n && w.Length >= m
+    requires v.Length <= 10 && w.Length <= 10
+    ensures b <==> forall k:: 0 <= k < n ==> exists x :: 0 <= x < m && v[k] == w[x]
+{
+	  var i: int := 0;
+	  var j: int := 0;
+
+	  while (i < n andalso j < m andalso (v[i] >= w[j]))
+	      invariant 0 <= i <= n
+	      invariant 0 <= j <= m
+        invariant forall k :: 0 <= k < i ==> (exists x:: 0 <= x < j && v[k] == w[x]) 
+	      invariant i < n ==> !(exists x:: 0 <= x < j && v[i] == w[x]) 
+        // dafny may not need these
+        invariant strictSorted(v)
+	      invariant strictSorted(w)
+        invariant n <= m && n >= 0
+        invariant v.Length >= n && w.Length >= m
+	  {	
+	  	  if(v[i] == w[j]){
+	  	  	  i:=i+1;
+	  	  }
+	  	  j:=j+1;
+	  }
+
+    if (i == n){
+        b := true;
+    }
+    else{
+        b := false;
+    }
+}
+
+predicate beq2(a: array<int>, b: array<int>, k1: int, k2: int)
+{
+    forall i :: 0 <= k1 <= i <= k2 < a.Length && k2 < b.Length  ==> a[i] == b[i]
+}
+
+method MergeSort_Incorrect(a0: array<int>) returns (a: array<int>) //this succeeds
+    requires 0 <= a0.Length <= 10 
+    ensures sorted(a, 0, a.Length - 1)
+{
+    a := ms_Incorrect(a0, 0, a0.Length - 1);
+}
+
+method ms_Incorrect(a0: array<int>, l : int, u : int) returns (a : array<int>) //this succeeds
+    requires 0 <= l && u < a0.Length && 0 <= a0.Length <= 10 
+    ensures a.Length == a0.Length
+    ensures beq2(a, a0, 0, l - 1) 
+    ensures beq2(a, a0, u + 1, a0.Length - 1)
+    ensures sorted(a, l, u)
+{
+    var m : int; 
+    a := a0; 
+    if (l >= u) { return a; }
+    else {
+        m := (l + u) / 2; 
+        a := ms_Incorrect(a, l, m); 
+        a := ms_Incorrect(a, m + 1, u); 
+        a := merge_Incorrect(a, l, m, u); 
+        return a; 
+    }
+}
+
+method merge_Incorrect(a0 : array<int>, l : int, m : int, u : int) returns (a : array<int>)
+    requires 0 <= a0.Length <= 10 && 0 <= l <= u < a0.Length && m == (l + u) / 2 
+    requires sorted (a0, l, m)
+    requires sorted (a0, m + 1, u)
+    ensures a.Length == a0.Length
+    ensures sorted (a, l, u)
+    ensures beq2(a, a0, 0, l - 1)
+    ensures beq2(a, a0, u + 1, a0.Length - 1)
+{
+    var i : int; 
+    var j : int; 
+    var k : int; 
+    var buf: array<int>; 
+
+    a := a0; 
+    buf := new [u - l + 1]; 
+    i := l; 
+    j := m + 1;
+
+    k := 0; 
+
+    while (k < buf.Length)
+        invariant l <= i <= m + 1
+        invariant m + 1 <= j <= u + 1
+        invariant 0 <= k <= buf.Length
+        //invariant k == (i - l) + (j - (m + 1))
+        invariant forall x:: 0 <= x < k && i <= m ==> buf[x] <= a[i] 
+        invariant forall x:: 0 <= x < k && j <= u ==> buf[x] <= a[j] 
+        invariant sorted (buf, 0, k - 1)
+        // dafny may not need these
+        invariant buf.Length == u - l + 1
+        invariant a.Length == a0.Length
+        invariant beq2 (a, a0, 0, a.Length - 1)
+        invariant 0 <= a0.Length <= 10 && 0 <= l <= u < a0.Length && m == (l + u) / 2
+        invariant sorted (a0, l, m)
+        invariant sorted (a0, m + 1, u)
+    {
+        if (i > m) { 
+          buf[k] := a[j]; 
+          j := j + 1;
+        } else if (j > u) { 
+          buf[k] := a[i]; 
+          i := i + 1;
+        } else if (a[i] <= a[j]) { 
+          buf[k] := a[i]; 
+          i := i + 1;
+        } else {
+          buf[k] := a[j]; 
+          j := j + 1;
+        }
+        k := k + 1;
+    }
+
+    k := 0;
+
+    while (k < buf.Length)
+        invariant 0 <= k && k <= buf.Length
+        invariant beq2(a, a0, 0, l - 1)
+        invariant beq2(a, a0, u + 1, a0.Length - 1)
+        invariant forall x :: 0 <= x < k ==> a[l + x] == buf[x]
+        invariant sorted(a, l, l + k - 1)
+        invariant sorted (buf, 0, buf.Length - 1) 
+        // dafny may not need these
+        invariant buf.Length == u - l + 1
+        invariant a.Length == a0.Length
+        invariant 0 <= a0.Length <= 10 && 0 <= l <= u < a0.Length && m == (l + u) / 2
+        invariant sorted (a0, l, m)
+        invariant sorted (a0, m + 1, u)
+    {
+        a[l + k] := buf[k];
+        k := k + 1;
+    }
+
+    return a; 
+}
+
+method MergeSort_Correct(a0: array<int>) returns (a: array<int>)
+    requires 0 <= a0.Length <= 10 
+    ensures sorted(a, 0, a.Length - 1)
+{
+    a := ms_Correct(a0, 0, a0.Length - 1);
+}
+
+method ms_Correct(a0: array<int>, l : int, u : int) returns (a : array<int>) 
+    requires 0 <= l && u < a0.Length && 0 <= a0.Length <= 10 
+    ensures a.Length == a0.Length
+    ensures beq2(a, a0, 0, l - 1) 
+    ensures beq2(a, a0, u + 1, a0.Length - 1)
+    ensures sorted(a, l, u)
+{
+    var m : int; 
+    a := a0; 
+    if (l >= u) { return a; }
+    else {
+      m := (l + u) / 2; 
+      a := ms_Correct(a, l, m); 
+      a := ms_Correct(a, m + 1, u); 
+      a := merge_Correct(a, l, m, u); 
+      return a; 
+    }
+}
+
+method merge_Correct(a0 : array<int>, l : int, m : int, u : int) returns (a : array<int>)
+    requires 0 <= a0.Length <= 10 && 0 <= l <= u < a0.Length && m == (l + u) / 2 
+    requires sorted (a0, l, m)
+    requires sorted (a0, m + 1, u)
+    ensures a.Length == a0.Length
+    ensures sorted (a, l, u)
+    ensures beq2(a, a0, 0, l - 1)
+    ensures beq2(a, a0, u + 1, a0.Length - 1)
+{
+    var i : int; 
+    var j : int; 
+    var k : int; 
+    var buf: array<int>; 
+
+    a := a0; 
+    buf := new [u - l + 1]; 
+    i := l; 
+    j := m + 1;
+
+    k := 0; 
+
+    while (k < buf.Length)
+        invariant l <= i <= m + 1
+        invariant m + 1 <= j <= u + 1
+        invariant 0 <= k <= buf.Length
+        invariant k == (i - l) + (j - (m + 1))
+        invariant forall x:: 0 <= x < k && i <= m ==> buf[x] <= a[i] 
+        invariant forall x:: 0 <= x < k && j <= u ==> buf[x] <= a[j] 
+        invariant sorted (buf, 0, k - 1)
+        // dafny may not need these
+        invariant buf.Length == u - l + 1
+        invariant a.Length == a0.Length
+        invariant beq2 (a, a0, 0, a.Length - 1)
+        invariant 0 <= a0.Length <= 10 && 0 <= l <= u < a0.Length && m == (l + u) / 2
+        invariant sorted (a0, l, m)
+        invariant sorted (a0, m + 1, u)
+    {
+        if (i > m) { 
+            buf[k] := a[j]; 
+            j := j + 1;
+        } else if (j > u) { 
+            buf[k] := a[i]; 
+            i := i + 1;
+        } else if (a[i] <= a[j]) { 
+            buf[k] := a[i]; 
+            i := i + 1;
+        } else {
+            buf[k] := a[j]; 
+            j := j + 1;
+        }
+        k := k + 1;
+    }
+
+    k := 0;
+
+    while (k < buf.Length)
+        invariant 0 <= k && k <= buf.Length
+        invariant beq2(a, a0, 0, l - 1)
+        invariant beq2(a, a0, u + 1, a0.Length - 1)
+        invariant forall x :: 0 <= x < k ==> a[l + x] == buf[x]
+        invariant sorted(a, l, l + k - 1)
+        invariant sorted (buf, 0, buf.Length - 1) 
+        // dafny may not need these
+        invariant buf.Length == u - l + 1
+        invariant a.Length == a0.Length
+        invariant 0 <= a0.Length <= 10 && 0 <= l <= u < a0.Length && m == (l + u) / 2
+        invariant sorted (a0, l, m)
+        invariant sorted (a0, m + 1, u)
+    {
+        a[l + k] := buf[k];
+        k := k + 1;
+    }
+
+    return a; 
+}
